Examples/RegSpec.v
@@ -7,164 +7,21 @@ From LHL.Util Require Import
   Tactics
   Util.
 
+From LHL.Examples Require Import
+  AtomicSpec.
+
 Variant RegSig {A} : ESig :=
 | Write (x : A) : RegSig unit
 | Read : RegSig A.
 Arguments RegSig : clear implicits.
 
-Variant RegState {T A} :=
-| RegDef (x : A) (m : option (Name T * {R & RegSig A R})).
-Arguments RegState : clear implicits.
-
-Arguments existT {A} {P}.
-
-Variant RegStep {T A} : RegState T A -> ThreadEvent T (RegSig A) -> RegState T A -> Prop :=
-| RegCall i x R (m : RegSig A R) :
-  RegStep (RegDef x None)
-          (i, CallEv m)
-          (RegDef x (Some (i, existT _ m)))
-| RetRetWrite i x y :
-  RegStep (RegDef x (Some (i, existT _ (Write y))))
-          (i, RetEv (Write y) tt)
-          (RegDef y None)
-| RegRetRead i x :
-  RegStep (RegDef x (Some (i, existT _ Read)))
-          (i, RetEv Read x)
-          (RegDef x None).
-
-Require Import Coq.Lists.List.
-Import ListNotations.
-
-Lemma double_ind {A} :
-  forall (P : list A -> Prop),
-  P [] ->
-  (forall x, P [x]) ->
-  (forall x y xs, P xs -> P (x :: y :: xs)) ->
-  forall xs,
-  P xs.
-intros.
-generalize dependent xs.
-fix rec 1.
-intros.
-destruct xs.
-{ apply H. }
-destruct xs.
-{ apply H0. }
-{
-  apply H1.
-  apply rec.
-}
-Qed.
-
-Require Import Coq.Logic.FunctionalExtensionality.
-
-Lemma regSeqCons {T A} init :
-  forall (p : list (ThreadEvent T (RegSig A))) (s : RegState T A),
-    Steps RegStep (RegDef init None) p s ->
-    SeqConsistent (fun _ : Name T => None) p.
-intros.
-revert H.
-generalize dependent init.
-change (
-  forall init,
-  Steps RegStep (RegDef init None) p s -> SeqConsistent (fun _ : Name T => None) p
-) with (
-  (fun p =>
-    forall init,
-    Steps RegStep (RegDef init None) p s -> SeqConsistent (fun _ : Name T => None) p
-  ) p
-).
-apply double_ind; intros.
-{ constructor. }
-{
-  ddestruct H.
-  ddestruct H.
-  eapply SCCall with
-    (a':=fun j =>
-      if i =? j then
-        Some (existT _ m)
-      else
-        (fun _ : Name T => None) j).
-  { easy. }
-  { now rewrite eqb_id. }
-  { apply differ_pointwise_trivial. }
-  { constructor. }
-}
-{
-  ddestruct H0. ddestruct H0.
-  eapply SCCall with
-    (a':=fun j =>
-      if i =? j then
-        Some (existT _ m)
-      else
-        (fun _ : Name T => None) j).
-  { easy. }
-  { now rewrite eqb_id. }
-  { apply differ_pointwise_trivial. }
-  ddestruct H1. ddestruct H0.
-  eapply SCRet with
-    (a':=fun j =>
-      if i =? j then
-        None
-      else if i =? j then
-        Some (existT _ (Write y))
-      else
-        (fun _ : Name T => None) j).
-  { now rewrite eqb_id. }
-  { now rewrite eqb_id. }
-  { apply differ_pointwise_trivial. }
-  assert (
-    (fun j : Name T =>
-      if i =? j then
-        None
-      else if i =? j then
-        Some (existT (P:=RegSig A) unit (Write y))
-      else None
-    ) = (fun _ => None)
-  ).
-  {
-    extensionality j.
-    dec_eq_nats i j.
-    { now rewrite eqb_id. }
-    { now rewrite eqb_nid. }
-  }
-  rewrite H0 at 1.
-  eapply H. exact H1.
-  eapply SCRet with
-    (a':=fun j =>
-      if i =? j then
-        None
-      else if i =? j then
-        Some (existT _ Read)
-      else
-        (fun _ : Name T => None) j).
-  { now rewrite eqb_id. }
-  { now rewrite eqb_id. }
-  { apply differ_pointwise_trivial. }
-  assert (
-    (fun j : Name T =>
-      if i =? j then
-        None
-      else if i =? j then
-        Some (existT (P:=RegSig R) _ Read)
-      else None
-    ) = (fun _ => None)
-  ).
-  {
-    extensionality j.
-    dec_eq_nats i j.
-    { now rewrite eqb_id. }
-    { now rewrite eqb_nid. }
-  }
-  rewrite H0 at 1.
-  eapply H. exact H1.
-}
-Qed.
+Variant RegStep {T A} : A -> Name T * {R & prod (RegSig A R) R} -> A -> Prop :=
+| RegRead i x : RegStep x (i, existT _ _ (Read, x)) x
+| RegWrite i x y : RegStep x (i, existT _ _ (Write y, tt)) y.
 
 Definition regSpec {T A} (init : A)
-: Spec T (RegSig A) := {|
-  State := RegState T A;
-  Step := RegStep;
-  Init := RegDef init None;
-  seq_cons := regSeqCons init
+: AtomicSpec T (RegSig A) := {|
+  AState := A;
+  AStep := RegStep;
+  AInit := init
 |}.
