Util/Util.v
@@ -6,6 +6,8 @@ From Coq Require Import
 From LHL.Util Require Import
   Tactics.
 
+Set Universe Polymorphism.
+
 Notation IRel M N := (forall X, M X -> N X -> Prop) (only parsing).
 
 Definition ieq {M : Type -> Type} R (e1 e2 : M R) : Prop := e1 = e2.
